coq/default.nix
@@ -2,9 +2,9 @@ let
   pkgs = import <nixpkgs>{}; 
 in 
 { stdenv ? pkgs.stdenv,
-  coq ? pkgs.coqPackages.coq,
+  coq ? pkgs.coq_8_13,
   gnumake ? pkgs.gnumake,
-  coqPackages ? pkgs.coqPackages,
+  coqPackages ? pkgs.coqPackages_8_13,
   ncurses ? pkgs.ncurses,
   which ? pkgs.which,
   graphviz ? pkgs.graphviz,
